specs/ecc/Spec.EC.Projective.Lemmas.fst
@@ -24,3 +24,32 @@ let lemma_proj_aff_id k p =
   M.lemma_div_mod_prime_one #prime pX;
   M.lemma_div_mod_prime_one #prime pY;
   assert (rx = pX /\ ry = pY)
+
+
+let to_aff_point_at_infinity_lemma k =
+  let px, py = to_aff_point k (point_at_inf k) in
+  assert (px == fmul k 0 (finv k 0) /\ py == fmul k 1 (finv k 0));
+  assert (px == fmul k 0 (M.pow_mod #prime 0 (prime - 2)));
+  M.lemma_pow_mod #prime 0 (prime - 2);
+  assert (px == fmul k 0 (M.pow 0 (prime - 2) % prime));
+  M.lemma_pow_zero (prime - 2);
+  assert (px == 0 /\ py == 0)
+
+
+let to_aff_point_negate_lemma k p =
+  let px, py, pz = p in
+  let qx, qy = to_aff_point k (point_negate k p) in
+  assert (qx == fmul k px (finv k pz) /\ qy == fmul k ((- py) % prime) (finv k pz));
+  let ax, ay = aff_point_negate k (to_aff_point k p) in
+  assert (ax == fmul k px (finv k pz) /\ ay == (- (fmul k py (finv k pz))) % prime);
+  let pz_inv = M.pow_mod #prime pz (prime - 2) in
+
+  calc (==) { // (-py) % prime /% pz;
+    ((- py) % k.prime * pz_inv) % k.prime;
+    (==) { Math.Lemmas.lemma_mod_mul_distr_l (- py) pz_inv k.prime }
+    ((- py) * pz_inv) % k.prime;
+    (==) { Math.Lemmas.neg_mul_left py pz_inv }
+    (- (py * pz_inv)) % k.prime;
+    (==) { Math.Lemmas.lemma_mod_sub_distr 0 (py * pz_inv) k.prime }
+    (- (py * pz_inv) % k.prime) % k.prime; // (- py /% pz) % prime;
+  }
