specs/lemmas/Spec.P256.Lemmas.fst
@@ -7,8 +7,6 @@ module M = Lib.NatMod
 
 #set-options "--z3rlimit 50 --ifuel 0 --fuel 0"
 
-let to_aff_point_at_infinity_lemma () = admit()
-
 let to_aff_point_add_lemma p q = admit()
 
 let to_aff_point_double_lemma p = admit()
